coqimp/contextswitch/proof/RegSaveProof.v
@@ -1,0 +1,111 @@
+Require Import Coqlib.                                                               
+Require Import Maps.            
+Require Import LibTactics.   
+        
+Require Import Integers.  
+Open Scope Z_scope.        
+Import ListNotations.  
+   
+Set Asymmetric Patterns.  
+        
+Require Import state.    
+Require Import language.  
+ 
+Set Implicit Arguments.    
+Unset Strict Implicit. 
+               
+Require Import logic.
+    
+Require Import lemmas.
+Require Import lemmas_ins.
+
+Require Import Coq.Logic.FunctionalExtensionality.
+
+Require Import integer_lemma.
+
+Require Import sep_lemma.
+Require Import reg_lemma.
+Require Import derived_rule.
+
+Require Import tm_dly_lemma.
+
+Require Import code.
+Require Import ctxswitch_spec.
+
+Require Import lemma1.
+
+Open Scope nat.
+Open Scope code_scope.
+Open Scope mem_scope.
+
+Theorem RegSaveProof :
+  forall vl,
+    spec |- {{ reg_save_pre vl }}
+             regsave
+           {{ reg_save_post vl }}.
+Proof.
+  intros.
+  unfold reg_save_pre.
+  unfold reg_save_post.
+  hoare_ex_intro_pre.
+  eapply Pure_intro_rule.
+  introv Hlgvl.
+  renames x' to fmg, x'0 to fmo, x'1 to fml, x'2 to fmi.
+  renames x'3 to ctx, x'5 to vy, x'7 to id, x'8 to vi, x'9 to F.
+  renames x'4 to l, x'6 to retf.
+  hoare_lift_pre 5.
+  eapply Pure_intro_rule.
+  introv Hpure.
+  destruct Hpure as [Hsp [Hctx_addr Hretf] ].
+  destruct fmg, fmo, fml, fmi.
+  simpl in Hsp.
+  simpl in Hretf.
+  inversion Hsp; subst.
+  inversion Hretf; subst.
+  destruct ctx as [l ctx].
+  simpl get_ctx_addr.
+  Print context.
+  destruct ctx as [ [ [rl ri] rg] ry].
+  hoare_lift_pre 2.
+  unfold context at 1.
+  unfold context' at 1.
+  eapply backward_rule.
+  introv Hs.
+  asrt_to_line_in Hs 3.
+  eauto.
+  unfold regsave.
+
+  Ltac save_reg_unfold' n m rls :=
+    match n with
+    | 0%nat =>
+      destruct rls as [ | ?a rls];
+      [idtac | ]
+    | S ?n' =>
+      destruct rls as [ | ?a rls];
+      [
+        let H := fresh in
+        simpl save_reg at 1; eapply backward_rule;
+        [
+          introv H; asrt_to_line_in H m;
+          simpl_sep_liftn_in H m; eapply H |
+          eapply Afalse_sep_rule] |
+        save_reg_unfold' n' (S m) rls
+      ]
+    end.
+      
+  Ltac save_reg_unfold :=
+    match goal with
+    | |- _ |- {{ save_reg ?l ?n ?rls ** ?p }} _ {{ _ }} =>
+      save_reg_unfold' n 1 rls
+    | _ => idtac
+    end.
+
+  save_reg_unfold.
+  destruct rl.
+  Focus 2.
+  simpl save_reg at 1.
+  
+  (** st l1 (l5 + OS_L1_OFFSET) *)
+  unfold OS_L1_OFFSET.
+  
+  
